core/Negation.thy
@@ -1,8 +1,12 @@
-section\<open>Core data structures\<close>
+section \<open>Negation procedure\<close>
 theory Negation
 imports Data Evaluate
 begin
-  
+
+text \<open>To compute the negation of a function f one merely needs to flip the values in the leaves.
+      Hence, one should be able to merely lazily remap the original BDD nodes into the same with
+      leaves negated.\<close>
+
 fun negate :: \<open>'l node \<Rightarrow> 'l node\<close> where
   \<open>negate (N u l h) = (let l' = (case l of Leaf b \<Rightarrow> Leaf (\<not>b) | _ \<Rightarrow> l)
                          ; h' = (case h of Leaf b \<Rightarrow> Leaf (\<not>b) | _ \<Rightarrow> h)
@@ -13,9 +17,9 @@ fun bdd_not :: \<open>'l bdd \<Rightarrow> 'l bdd\<close> where
 | \<open>bdd_not (Nodes ns)   = (Nodes (map negate ns))\<close>
 
 lemma bdd_not_correct_aux:
-  assumes \<open>well_formed_nl ns\<close> \<open>t \<in> uid ` set ns\<close>
-  shows \<open>\<not>bdd_eval_aux ns a t \<longleftrightarrow> bdd_eval_aux (map negate ns) a t\<close>
-  using assms by (induction ns arbitrary: t rule: nl_induct) (auto split: ptr.splits)
+  assumes \<open>well_formed_nl ns\<close> \<open>tgt \<in> uid ` set ns\<close>
+  shows \<open>\<not>bdd_eval_node ns a tgt \<longleftrightarrow> bdd_eval_node (map negate ns) a tgt\<close>
+  using assms by (induction ns arbitrary: tgt rule: nl_induct) (auto split: ptr.splits)  
 
 theorem bdd_not_correct:
   assumes \<open>well_formed bdd\<close>
